ironfleet/src/Dafny/Distributed/Services/WS/WS.s.dfy
@@ -5,20 +5,34 @@ module WS__WS_s {
 import opened Native__Io_s
 
 type HTTPRequest = seq<char>
-datatype HTTPResponse = ResponseValid(r:seq<byte>) | Response404()
+type HTTPResponse = seq<byte>
 
 predicate SpecInit()
 {
     true
 }
 
+// supports only a very primitive request format at the moment
+predicate IsValidHTTPReq(req:HTTPRequest)
+{
+    exists op,filePath,ver :: (req == op + " " + filePath + " " + ver) 
+                               && op == "GET" && |filePath| > 1 
+                               && ver == "HTTP/1.0" 
+}
+
+// TODO: HTTP response should include headers
 predicate Get(fs:FileSystemState, req:HTTPRequest, res:HTTPResponse)
     requires fs != null;
 {
+       // Is there a way to avoid duplicating this?
        fs != null
-    && (exists op,filePath,ver :: (req == op + " " + filePath + " " + ver) 
+    && if IsValidHTTPReq(req) then
+        (exists op,filePath,ver :: (req == op + " " + filePath + " " + ver) 
                                && op == "GET" && |filePath| > 1 
                                && ver == "HTTP/1.0" 
-                               && (res == if fs.file_exists(filePath) then ResponseValid(fs.contents(filePath[1..])) else Response404()))
+                               && (res == if fs.file_exists(filePath) then fs.contents(filePath[1..]) else []))
+       else
+        res == []
+         
 }
 }
